src/Step.v
@@ -1,0 +1,272 @@
+From Heapster Require Import
+     Config.
+
+From Coq Require Import
+     Structures.Equalities
+     Ensembles
+     Classes.Morphisms
+     Classes.RelationClasses
+     Relations.Relation_Operators
+     Relations.Operators_Properties
+     Program.Equality.
+
+From ExtLib Require Import
+     Structures.Functor
+     Structures.Monad.
+
+From ITree Require Import
+     ITree
+     ITreeFacts
+     Basics.MonadState
+     Basics.MonadProp
+     Events.State
+     Events.Nondeterminism
+     Eq.Eq
+     Eq.UpToTaus
+     Eq.EqAxiom.
+
+From Paco Require Import
+     paco.
+
+Import ITreeNotations.
+Open Scope monad_scope.
+
+Variant MemoryE : Type -> Type :=
+| Load : forall (p : SByte), MemoryE SByte
+| Store : forall (p v : SByte) , MemoryE unit
+.
+
+(* Definition E := (stateE config +' nondetE). *)
+Definition E := (MemoryE +' nondetE).
+
+Variant step {R} : itree E R -> config -> itree E R -> config -> Prop :=
+| step_tau : forall t c, step (Tau t) c t c
+| step_nondet_true : forall k c, step (vis Or k) c (k true) c
+| step_nondet_false : forall k c, step (vis Or k) c (k false) c
+| step_load : forall k c p v, read c p = Some v ->
+                         step (vis (Load (Ptr p)) k) c (k v) c
+| step_store : forall k c c' p v, write c p v = Some c' ->
+                             step (vis (Store (Ptr p) v) k) c (k tt) c'
+| step_load_fail : forall k c p, read c p = None ->
+                            step (vis (Load (Ptr p)) k) c (k (Byte 0)) (error_config c)
+| step_store_fail : forall k c p v, write c p v = None ->
+                               step (vis (Store (Ptr p) v) k) c (k tt) (error_config c)
+(* | step_get : forall k c, step (vis (Get _) k) c (k c) c *)
+(* | step_put : forall k c c', step (vis (Put _ c') k) c (k tt) c' *)
+.
+
+Inductive multistep {R} : itree E R -> config -> itree E R -> config -> Prop :=
+| multistep_refl : forall t c, multistep t c t c
+| multistep_step : forall t c t' c' t'' c'',
+    multistep t c t' c' -> step t' c' t'' c'' -> multistep t c t'' c''
+.
+
+Ltac rewritebisim lem := pose proof lem as bisim;
+                         eapply bisimulation_is_eq in bisim;
+                         rewrite bisim;
+                         clear bisim.
+
+Ltac rewritebisim_in lem H := pose proof lem as bisim;
+                              eapply bisimulation_is_eq in bisim;
+                              rewrite bisim in H;
+                              clear bisim.
+
+Lemma step_bind {R1 R2} : forall (t1 t2 : itree E R1) (c1 c2 : config) (k : R1 -> itree E R2),
+    step t1 c1 t2 c2 ->
+    step (t1 >>= k) c1 (t2 >>= k) c2.
+Proof.
+  intros. inversion H; subst; try solve [rewritebisim @bind_vis; constructor; auto].
+  - rewritebisim @bind_tau. constructor.
+  - rewritebisim @bind_vis.
+    (* constructor doesn't work here for some reason *)
+    apply (step_load (fun v => x <- k0 v;; k x) _ _ _ H0).
+Qed.
+
+Lemma step_ret_bind {R1 R2} : forall (t1 t2 : itree E R1) (c1 c2 : config) (r : R2),
+    step t1 c1 t2 c2 ->
+    step (Ret r;; t1) c1 t2 c2.
+Proof.
+  intros. rewritebisim @bind_ret_l. assumption.
+Qed.
+
+Lemma step_fmap {R1 R2} : forall (t t' : itree E R1) c c' (f : R1 -> R2),
+    step t c t' c' ->
+    step (fmap f t) c (fmap f t') c'.
+Proof.
+  intros. inversion H; subst; simpl; unfold ITree.map;
+            try solve [rewritebisim @bind_vis; constructor; auto].
+  - rewritebisim @bind_tau. constructor; auto.
+  - rewritebisim @bind_vis.
+    (* again have to specify k manually? *)
+    apply (step_load (fun x => x' <- k x;; Ret (f x'))); auto.
+Qed.
+
+Lemma bind_fst {R1 R2} (t : itree E R1) (r2 : R2) :
+  x1 <- t;; x <- Ret (x1, r2);; Ret (fst x) ≅ t.
+Proof.
+  revert t r2. pcofix CIH. intros.
+  rewritebisim @unfold_bind. pstep.
+  rewrite (itree_eta_ t0). destruct (observe t0); simpl.
+  - rewritebisim @unfold_bind. constructor; auto.
+  - constructor; auto.
+  - constructor; auto.
+Qed.
+
+Lemma bind_snd {R1 R2} (t : itree E R2) (r1 : R1) :
+  x2 <- t;; x <- Ret (r1, x2);; Ret (snd x) ≅ t.
+Proof.
+  revert t r1. pcofix CIH. intros.
+  rewritebisim @unfold_bind. pstep.
+  rewrite (itree_eta_ t0). destruct (observe t0); simpl.
+  - rewritebisim @unfold_bind. constructor; auto.
+  - constructor; auto.
+  - constructor; auto.
+Qed.
+
+Lemma step_fmap_fst {R1 R2} : forall (t : itree E R2) (t' : itree E (R1 * R2)) c c' (r1 : R1),
+    step (fmap (fun r2 : R2 => (r1, r2)) t) c t' c' ->
+    step t c (fmap snd t') c'.
+Proof.
+  simpl. intros. unfold ITree.map in *. inversion H; subst.
+  - edestruct @eqitree_inv_bind_tau as [(? & ? & ?) | (? & ? & ?)];
+      [rewrite H1; reflexivity | |].
+    + apply bisimulation_is_eq in H0. apply bisimulation_is_eq in H2.
+      rewrite H0. rewrite <- H2. rewritebisim @bind_bind. rewritebisim @bind_snd. constructor.
+    + apply bisimulation_is_eq in H0. rewrite H0 in H1.
+      rewritebisim_in @bind_ret_l H1. inversion H1.
+  - edestruct @eqitree_inv_bind_vis as [(? & ? & ?) | (? & ? & ?)];
+      [rewrite H1; reflexivity | |].
+    + specialize (H2 true). apply bisimulation_is_eq in H0. apply bisimulation_is_eq in H2.
+      rewrite H0. rewrite <- H2. rewritebisim @bind_bind. rewritebisim @bind_snd. constructor.
+    + apply bisimulation_is_eq in H0. rewrite H0 in H1.
+      rewritebisim_in @bind_ret_l H1. inversion H1.
+  - edestruct @eqitree_inv_bind_vis as [(? & ? & ?) | (? & ? & ?)];
+      [rewrite H1; reflexivity | |].
+    + specialize (H2 false). apply bisimulation_is_eq in H0. apply bisimulation_is_eq in H2.
+      rewrite H0. rewrite <- H2. rewritebisim @bind_bind. rewritebisim @bind_snd. constructor.
+    + apply bisimulation_is_eq in H0. rewrite H0 in H1.
+      rewritebisim_in @bind_ret_l H1. inversion H1.
+  - edestruct @eqitree_inv_bind_vis as [(? & ? & ?) | (? & ? & ?)];
+      [rewrite H0; reflexivity | |].
+    + specialize (H3 v). apply bisimulation_is_eq in H2. apply bisimulation_is_eq in H3.
+      rewrite H2. rewrite <- H3.
+      rewritebisim @bind_bind. rewritebisim @bind_snd. constructor; auto.
+    + apply bisimulation_is_eq in H2. rewrite H2 in H0.
+      rewritebisim_in @bind_ret_l H0. inversion H0.
+  - edestruct @eqitree_inv_bind_vis as [(? & ? & ?) | (? & ? & ?)];
+      [rewrite H0; reflexivity | |].
+    + specialize (H3 tt). apply bisimulation_is_eq in H2. apply bisimulation_is_eq in H3.
+      rewrite H2. rewrite <- H3.
+      rewritebisim @bind_bind. rewritebisim @bind_snd. constructor; auto.
+    + apply bisimulation_is_eq in H2. rewrite H2 in H0.
+      rewritebisim_in @bind_ret_l H0. inversion H0.
+  - edestruct @eqitree_inv_bind_vis as [(? & ? & ?) | (? & ? & ?)];
+      [rewrite H0; reflexivity | |].
+    + specialize (H3 (Byte 0)). apply bisimulation_is_eq in H2. apply bisimulation_is_eq in H3.
+      rewrite H2. rewrite <- H3.
+      rewritebisim @bind_bind. rewritebisim @bind_snd. constructor; auto.
+    + apply bisimulation_is_eq in H2. rewrite H2 in H0.
+      rewritebisim_in @bind_ret_l H0. inversion H0.
+  - edestruct @eqitree_inv_bind_vis as [(? & ? & ?) | (? & ? & ?)];
+      [rewrite H0; reflexivity | |].
+    + specialize (H3 tt). apply bisimulation_is_eq in H2. apply bisimulation_is_eq in H3.
+      rewrite H2. rewrite <- H3.
+      rewritebisim @bind_bind. rewritebisim @bind_snd. constructor 7; auto.
+    + apply bisimulation_is_eq in H2. rewrite H2 in H0.
+      rewritebisim_in @bind_ret_l H0. inversion H0.
+Qed.
+
+Lemma step_fmap_snd {R1 R2} : forall (t : itree E R1) (t' : itree E (R1 * R2)) c c' (r2 : R2),
+    step (fmap (fun r1 : R1 => (r1, r2)) t) c t' c' ->
+    step t c (fmap fst t') c'.
+Proof.
+  simpl. intros. unfold ITree.map in *. inversion H; subst.
+  - edestruct @eqitree_inv_bind_tau as [(? & ? & ?) | (? & ? & ?)];
+      [rewrite H1; reflexivity | |].
+    + apply bisimulation_is_eq in H0. apply bisimulation_is_eq in H2.
+      rewrite H0. rewrite <- H2. rewritebisim @bind_bind. rewritebisim @bind_fst. constructor.
+    + apply bisimulation_is_eq in H0. rewrite H0 in H1.
+      rewritebisim_in @bind_ret_l H1. inversion H1.
+  - edestruct @eqitree_inv_bind_vis as [(? & ? & ?) | (? & ? & ?)];
+      [rewrite H1; reflexivity | |].
+    + specialize (H2 true). apply bisimulation_is_eq in H0. apply bisimulation_is_eq in H2.
+      rewrite H0. rewrite <- H2. rewritebisim @bind_bind. rewritebisim @bind_fst. constructor.
+    + apply bisimulation_is_eq in H0. rewrite H0 in H1.
+      rewritebisim_in @bind_ret_l H1. inversion H1.
+  - edestruct @eqitree_inv_bind_vis as [(? & ? & ?) | (? & ? & ?)];
+      [rewrite H1; reflexivity | |].
+    + specialize (H2 false). apply bisimulation_is_eq in H0. apply bisimulation_is_eq in H2.
+      rewrite H0. rewrite <- H2. rewritebisim @bind_bind. rewritebisim @bind_fst. constructor.
+    + apply bisimulation_is_eq in H0. rewrite H0 in H1.
+      rewritebisim_in @bind_ret_l H1. inversion H1.
+  - edestruct @eqitree_inv_bind_vis as [(? & ? & ?) | (? & ? & ?)];
+      [rewrite H0; reflexivity | |].
+    + specialize (H3 v). apply bisimulation_is_eq in H2. apply bisimulation_is_eq in H3.
+      rewrite H2. rewrite <- H3.
+      rewritebisim @bind_bind. rewritebisim @bind_fst. constructor; auto.
+    + apply bisimulation_is_eq in H2. rewrite H2 in H0.
+      rewritebisim_in @bind_ret_l H0. inversion H0.
+  - edestruct @eqitree_inv_bind_vis as [(? & ? & ?) | (? & ? & ?)];
+      [rewrite H0; reflexivity | |].
+    + specialize (H3 tt). apply bisimulation_is_eq in H2. apply bisimulation_is_eq in H3.
+      rewrite H2. rewrite <- H3.
+      rewritebisim @bind_bind. rewritebisim @bind_fst. constructor; auto.
+    + apply bisimulation_is_eq in H2. rewrite H2 in H0.
+      rewritebisim_in @bind_ret_l H0. inversion H0.
+  - edestruct @eqitree_inv_bind_vis as [(? & ? & ?) | (? & ? & ?)];
+      [rewrite H0; reflexivity | |].
+    + specialize (H3 (Byte 0)). apply bisimulation_is_eq in H2. apply bisimulation_is_eq in H3.
+      rewrite H2. rewrite <- H3.
+      rewritebisim @bind_bind. rewritebisim @bind_fst. constructor; auto.
+    + apply bisimulation_is_eq in H2. rewrite H2 in H0.
+      rewritebisim_in @bind_ret_l H0. inversion H0.
+  - edestruct @eqitree_inv_bind_vis as [(? & ? & ?) | (? & ? & ?)];
+      [rewrite H0; reflexivity | |].
+    + specialize (H3 tt). apply bisimulation_is_eq in H2. apply bisimulation_is_eq in H3.
+      rewrite H2. rewrite <- H3.
+      rewritebisim @bind_bind. rewritebisim @bind_fst. constructor 7; auto.
+    + apply bisimulation_is_eq in H2. rewrite H2 in H0.
+      rewritebisim_in @bind_ret_l H0. inversion H0.
+Qed.
+
+Lemma step_fmap_inv {R1 R2 : Type} (f : R1 -> R2) (t : itree E R1) (t' : itree E R2) c c' :
+  step (fmap f t) c t' c' ->
+  exists t'', t' = fmap f t''.
+Proof.
+  intros. simpl in *. unfold ITree.map in *. inversion H; subst.
+  - edestruct @eqitree_inv_bind_tau as [(? & ? & ?) | (? & ? & ?)];
+      [rewrite H1; reflexivity | |].
+    + apply bisimulation_is_eq in H2. eexists. symmetry. apply H2.
+    + apply bisimulation_is_eq in H0. rewrite H0 in H1.
+      rewritebisim_in @bind_ret_l H1. inversion H1.
+  - edestruct @eqitree_inv_bind_vis as [(? & ? & ?) | (? & ? & ?)];
+      [rewrite H1; reflexivity | |].
+    + specialize (H2 true). apply bisimulation_is_eq in H2. eexists. symmetry. apply H2.
+    + apply bisimulation_is_eq in H0. rewrite H0 in H1.
+      rewritebisim_in @bind_ret_l H1. inversion H1.
+  - edestruct @eqitree_inv_bind_vis as [(? & ? & ?) | (? & ? & ?)];
+      [rewrite H1; reflexivity | |].
+    + specialize (H2 false). apply bisimulation_is_eq in H2. eexists. symmetry. apply H2.
+    + apply bisimulation_is_eq in H0. rewrite H0 in H1.
+      rewritebisim_in @bind_ret_l H1. inversion H1.
+  - edestruct @eqitree_inv_bind_vis as [(? & ? & ?) | (? & ? & ?)];
+      [rewrite H0; reflexivity | |].
+    + specialize (H3 v). apply bisimulation_is_eq in H3. eexists. symmetry. apply H3.
+    + apply bisimulation_is_eq in H2. rewrite H2 in H0.
+      rewritebisim_in @bind_ret_l H0. inversion H0.
+  - edestruct @eqitree_inv_bind_vis as [(? & ? & ?) | (? & ? & ?)];
+      [rewrite H0; reflexivity | |].
+    + specialize (H3 tt). apply bisimulation_is_eq in H3. eexists. symmetry. apply H3.
+    + apply bisimulation_is_eq in H2. rewrite H2 in H0.
+      rewritebisim_in @bind_ret_l H0. inversion H0.
+  - edestruct @eqitree_inv_bind_vis as [(? & ? & ?) | (? & ? & ?)];
+      [rewrite H0; reflexivity | |].
+    + specialize (H3 (Byte 0)). apply bisimulation_is_eq in H3. eexists. symmetry. apply H3.
+    + apply bisimulation_is_eq in H2. rewrite H2 in H0.
+      rewritebisim_in @bind_ret_l H0. inversion H0.
+  - edestruct @eqitree_inv_bind_vis as [(? & ? & ?) | (? & ? & ?)];
+      [rewrite H0; reflexivity | |].
+    + specialize (H3 tt). apply bisimulation_is_eq in H3. eexists. symmetry. apply H3.
+    + apply bisimulation_is_eq in H2. rewrite H2 in H0.
+      rewritebisim_in @bind_ret_l H0. inversion H0.
+Qed.
